Hoare rule for sequencing complete. But does not yet handle case of multiple simultaneous semantics for Seq.

CPS_Ctl/Seq.thy
@@ -27,7 +27,8 @@ definition seq_sem' :: "syn \<Rightarrow> 'x state' \<Rightarrow> 'x state'" whe
       Sskip \<Rightarrow> t
       | Sseq \<Rightarrow> l@t))"
 
-type_synonym 'x state = "'x gensyn list md_triv option md_prio"
+type_synonym 'x state = 
+  "('x, unit option) control"
 
 term "(schem_lift
     (SP NA (SP NB NC)) (SP (SO NA) (SP (SPRI (SO NB)) (SPRI (SO NC)))))"
@@ -36,7 +37,7 @@ term "(schem_lift
 definition seq_sem_lifting :: "(syn, 'x state', 'x state) lifting"
   where
 "seq_sem_lifting = schem_lift
-    NC (SPRI (SO NC)) "
+    NC (SP (SPRI (SO NC)) NX) "
 
 definition seq_sem_l :: "syn \<Rightarrow> 'x state \<Rightarrow> 'x state" where
 "seq_sem_l =
@@ -44,31 +45,81 @@ definition seq_sem_l :: "syn \<Rightarrow> 'x state \<Rightarrow> 'x state" wher
   seq_sem_lifting
   seq_sem'"
 
-definition seq_sem :: "(syn, 'x, 'x state) sem" where
+definition seq_sem :: "(syn, 'x, unit option) sem" where
 "seq_sem \<equiv>
-  \<lparr> s_sem = seq_sem_l
-  , s_l = seq_sem_lifting \<rparr>"
+  \<lparr> s_sem = seq_sem_l \<rparr>"
 
-definition seq_sem_l_gen ::
-  "('s \<Rightarrow> syn) \<Rightarrow>
-   (syn, 'x state', ('y :: Pord)) lifting \<Rightarrow>
-   's \<Rightarrow> 'y \<Rightarrow> 'y" where
-"seq_sem_l_gen lfts lft =
-  lift_map_s lfts
-  lft
-  seq_sem'"
 
 (* TODO: the next thing is making
    sure this all still works in the face of a true merge
    with multiple liftings. *)
+(* TODO: are all these parameters necessary?
+   ('s as well as 'x)
+*)
+
+(* this isn't quite right. we need to constrain the lifting so that the
+   control data is being lifted into the second component *)
+(*
 definition seq_semx :: 
 "('s \<Rightarrow> syn) \<Rightarrow>
- (syn, 'x state', ('y :: Pord)) lifting \<Rightarrow>
- ('s, 'x, ('y :: Pord)) sem" where
+ (syn, 'x state', ('x, 'z :: Pord) control) lifting \<Rightarrow>
+ ('s, 'x, 'z) sem" where
 "seq_semx lfts lft \<equiv>
-  \<lparr> s_sem = seq_sem_l_gen lfts lft
-  , s_l = l_synt lfts lft\<rparr>"
+  \<lparr> s_sem = seq_sem_l_gen lfts lft \<rparr>"
+*)
 
+
+(* TODO: see if there is a way to update the auto lifter so that
+   it works with parameterized stuff *)
+
+definition seq_sem_lifting_gen' :: "(syn, 'x state', ('x, 'y :: Pordb) control) lifting"
+  where
+"seq_sem_lifting_gen' = schem_lift
+    NC (SP (SPRI (SO NC)) NX) "
+
+term  "seq_sem_lifting_gen' :: (syn, unit state', (unit, unit option) control) lifting"
+
+definition seq_sem_lifting' :: "(syn, 'x state', 'x state' md_triv option md_prio) lifting"
+  where
+"seq_sem_lifting' =
+  (prio_l (\<lambda> _ . 0) (\<lambda> _ z . 1 + z) (option_l (triv_l)))"
+
+definition seq_sem_lifting_gen :: "(syn, 'x state', ('x, 'y :: Pordb) control) lifting"
+  where
+"seq_sem_lifting_gen = fst_l (seq_sem_lifting')"
+
+lemma fst_l_S_univ : 
+  "(fst_l_S (\<lambda> _ . UNIV)) = (\<lambda> _ . UNIV)"
+  unfolding fst_l_S_def
+  by(blast)
+
+lemma seq_sem_lifting_gen_validb :
+  "lifting_validb (seq_sem_lifting_gen :: (syn, 'x state', ('x, 'y :: Pordb) control) lifting) 
+                  (\<lambda> _ . UNIV)" unfolding seq_sem_lifting_gen_def
+  unfolding seq_sem_lifting'_def
+  apply(simp only: sym[OF fst_l_S_univ])
+  apply(rule fst_l_validb)
+  apply(rule prio_l_validb_strong)
+    apply(rule option_l_valid_weakb)
+    apply(rule triv_l_valid_weak)
+   apply(auto)
+  done
+
+
+definition seq_sem_l_gen ::
+  "('s \<Rightarrow> syn) \<Rightarrow>
+   's \<Rightarrow> (('x, 'y :: Pordb) control) \<Rightarrow> (('x, 'y :: Pordb) control)" where
+"seq_sem_l_gen lfts =
+  lift_map_s lfts
+  seq_sem_lifting_gen
+  seq_sem'"
+
+
+definition seq_semx :: 
+"('s \<Rightarrow> syn) \<Rightarrow>
+ ('s, 'x, 'z :: Pordb) sem" where
+"seq_semx lfts \<equiv>
+  \<lparr> s_sem = seq_sem_l_gen lfts \<rparr>"
 
 (* 
   question
@@ -81,9 +132,15 @@ GS, one for each sub-language
     - 
 *)
 
+(* TODO: this proof is currently rather nasty, as it
+   involves unfolding a bunch of liftings *)
+
+(* TODO: to use this with other rules, we'll need some notion of monotonicity of
+   control flow (i.e. continuation list). perhaps this can be built into
+   our Hoare abstraction?
+*)
 lemma HSeq :
-  assumes HV : "lifting_valid_weak lft Sv"
-  assumes H0 : "gs = seq_semx lfts lft"
+  assumes H0 : "gs = seq_semx lfts"
   assumes H1 : "lfts Sseq' = Sseq"
   assumes H : "|gs| {- P1 -} cs {- P2 -}"
   shows "|gs| {- P1 -} [G Sseq' cs] {- P2 -}"
@@ -97,45 +154,60 @@ proof
 
   show "|gs| {P1} [G Sseq' cs] @ c'"
   proof
-    fix m
-    assume M : "P1 m"
-    assume CM : "s_cont gs m = [G Sseq' cs] @ c'"
+    fix m :: "('a, 'b) control"
+    assume M : "P1 (snd m)"
+    assume CM : "s_cont m = [G Sseq' cs] @ c'"
 
-    obtain m1 where
-      Step : "sem_step_p gs m m1" and
-      CM1 : "s_cont gs m1 = cs @ c'"
-      using CM lifting_valid_weakDO[OF HV] unfolding H0
-      apply(simp add: sem_step_p_eq sem_step_def seq_semx_def seq_sem_l_gen_def seq_sem'_def l_synt_def s_cont_def H1)
 
-(* is lifting the right abstraction here?
-maybe we actually do want something different.
-but, if we can use existing lifting stuff that is a big win
-so i'm not ready to give up on using lifting as is, yet. *)
+(* lifting_validDI[OF lifting_validbDV[OF seq_sem_lifting_gen_validb]]  *)
 
-    have M1_eq : "LUpd lft Sseq (cs @ c') m = m1" using Step CM H1 unfolding sem_step_p_eq H0 CM
-      by(simp add: sem_step_p_eq sem_step_def seq_semx_def seq_sem_l_gen_def seq_sem'_def split: option.splits list.splits)
+    show "(safe gs m)"
+    proof(cases "(sem_step gs m)")
+      case None
 
-    (* need to put entire lifting into definition *)
-    have M1 : "P1 m1" sorry
+      then have False using CM H0
+        by(auto simp add: sem_step_def)
 
-    have Conc' : "safe gs m1" using guardedD[OF Guarded M1 CM1]
-      by auto
+      then show ?thesis by auto
+    next
+      case (Some m')
 
-    show "safe gs m"
-    proof
-      fix m'
-      assume XP : "sem_exec_p gs m m'"
-        
-      show "imm_safe gs m'" using XP unfolding sem_exec_p_def
-      proof(cases rule: rtranclp.cases)
-      case rtrancl_refl
-        then show ?thesis using imm_safeI_Step[OF Step] by auto
-      next
-        case RT : (rtrancl_into_rtrancl b)
+(*TODO: make this less bad *)
+      have CM1 :  "s_cont m' = cs @ c'"
+        using Some CM H0 H1
+        by(cases m; cases m'; auto simp add: sem_step_def seq_semx_def seq_sem_l_gen_def seq_sem'_def s_cont_def seq_sem_lifting_gen_def fst_l_def seq_sem_lifting'_def
+            prio_l_def option_l_def triv_l_def split: md_prio.splits option.splits md_triv.splits)
 
-        have Exc : "sem_exec_p gs m1 m'" unfolding sem_exec_p_def using rtranclp_bisect1[OF sem_step_determ RT(1) Step RT(2)] by auto
+(*TODO: make this less bad *)
+      have M1_eq : "snd m' = snd m"
+        using Some H0
+        by(cases m; cases m'; auto simp add: sem_step_def seq_semx_def seq_sem_l_gen_def seq_sem'_def s_cont_def seq_sem_lifting_gen_def fst_l_def seq_sem_lifting'_def
+            prio_l_def option_l_def triv_l_def split: md_prio.splits option.splits md_triv.splits list.split_asm)
 
-        then show ?thesis using safeD[OF Conc' Exc] by auto
+      have M1 : "P1 (snd m')" using M unfolding M1_eq by auto
+
+      have Step : "sem_step_p gs m m'"
+        using sem_step_sem_step_p[OF Some] by auto
+
+      have Conc' : "safe gs m'" using guardedD[OF Guarded M1 CM1]
+        by auto
+
+      show "safe gs m"
+      proof
+        fix m''
+        assume XP : "sem_exec_p gs m m''"
+          
+        show "imm_safe gs m''" using XP unfolding sem_exec_p_def
+        proof(cases rule: rtranclp.cases)
+        case rtrancl_refl
+          then show ?thesis using imm_safeI_Step[OF Step] by auto
+        next
+          case RT : (rtrancl_into_rtrancl b)
+  
+          have Exc : "sem_exec_p gs m' m''" unfolding sem_exec_p_def using rtranclp_bisect1[OF sem_step_determ RT(1) Step RT(2)] by auto
+  
+          then show ?thesis using safeD[OF Conc' Exc] by auto
+        qed
       qed
     qed
   qed
